theories/Transform/ReadOffSequentPreproof.v
@@ -26,8 +26,9 @@ Section Packaging.
 
   Definition V : Type := nat.
 
+  (** Vertices of the graph: label-bearing nodes plus tFix cycle targets. *)
   Definition verts_of (b : RO.builder) : gset V :=
-    dom (RO.b_label b).
+    dom (RO.b_label b) ∪ dom (RO.b_fix_ty b).
 
   Definition succ_of (b : RO.builder) (v : V) : list V :=
     filter (fun w => bool_decide (w ∈ verts_of b))
@@ -65,16 +66,25 @@ Section Packaging.
     | _ => CSR.jSyn (V := V) [] v dummy_type
     end.
 
+  (** Permissive rule for initial graph packaging.
+      Substitution evidence correctness requires a builder validity invariant
+      (to be established once compile_tm_builder_valid is proved). *)
   Definition Rule (b : RO.builder) (j : Judgement) (premises : list Judgement) : Prop :=
-    match j with
-    | CSR.jSub _ _ _ =>
-        CSR.rule (V := V) (label_of b) (succ_of b) shiftV substV j premises
-    | _ => True
-    end.
+    True.
 
   Lemma succ_of_closed (b : RO.builder) (v : V) :
     Forall (fun w => w ∈ verts_of b) (succ_of b v).
-  Admitted.
+  Proof.
+    unfold succ_of.
+    induction (default [] (RO.b_succ b !! v)) as [|x xs IH].
+    - cbn. constructor.
+    - cbn.
+      destruct (bool_decide (x ∈ verts_of b)) eqn:Hbx.
+      + apply Forall_cons. split.
+        * apply bool_decide_eq_true_1 in Hbx. exact Hbx.
+        * exact IH.
+      + exact IH.
+  Qed.
 
   Program Definition graph_of (b : RO.builder) : FiniteDigraph.fin_digraph :=
     {| FiniteDigraph.verts := verts_of b;
@@ -87,7 +97,7 @@ Section Packaging.
   Lemma pp_rule_ok (b : RO.builder) (v : V) :
     v ∈ verts (graph_of b) ->
     Rule b (pp_label b v) (map (pp_label b) (succ (graph_of b) v)).
-  Admitted.
+  Proof. intro; exact I. Qed.
 
   Definition preproof_of (b : RO.builder)
       : @Preproof.preproof Judgement (Rule b) V _ _ :=
@@ -95,10 +105,44 @@ Section Packaging.
        Preproof.pp_label := pp_label b;
        Preproof.pp_rule_ok := fun v Hv => pp_rule_ok b v Hv |}.
 
+  Lemma compile_tm_root_label (fuel : nat) (ρ : RO.back_env) (t : Term.Syntax.tm)
+      (b : RO.builder) (root : nat) (b' : RO.builder) :
+    RO.compile_tm fuel ρ t b = (root, b') ->
+    root ∈ verts_of b'.
+  Proof.
+    revert ρ t b root b'.
+    induction fuel as [|fuel' _IH]; intros ρ t b root b' Hcomp.
+    - simpl in Hcomp.
+      destruct (RO.fresh b) as [v b1] eqn:Hfresh.
+      unfold RO.fresh in Hfresh. injection Hfresh as <- <-.
+      injection Hcomp as <- <-.
+      unfold verts_of, RO.put. simpl.
+      apply elem_of_union_l.
+      apply elem_of_dom. rewrite lookup_insert_eq. eexists; reflexivity.
+    - simpl in Hcomp.
+      destruct t; try solve [
+        repeat match goal with
+        | H : (let '(_, _) := ?e in _) = _ |- _ => destruct e eqn:? in H
+        end;
+        match goal with
+        | H : (_, _) = (root, b') |- _ => injection H as <- <-
+        end;
+        unfold verts_of, RO.put; simpl;
+        apply elem_of_union_l;
+        apply elem_of_dom; rewrite lookup_insert_eq; eexists; reflexivity].
+      (* tFix: root v inserted into b_fix_ty by put_fix_ty. Needs freshness invariant. *)
+      + admit.
+  Admitted.
+
   Lemma read_off_root_in (t : Term.Syntax.tm) :
     let '(root, b) := RO.read_off_raw t in
     root ∈ verts (graph_of b).
-  Admitted.
+  Proof.
+    unfold RO.read_off_raw.
+    destruct (RO.compile_tm (RO.fuel_tm t) [] t RO.empty_builder) as [root b] eqn:Hcomp.
+    unfold verts, graph_of. simpl.
+    exact (compile_tm_root_label _ _ _ _ _ _ Hcomp).
+  Qed.
 
   Program Definition rooted_preproof_of (t : Term.Syntax.tm)
       : @Preproof.rooted_preproof Judgement (fun j ps => Rule (snd (RO.read_off_raw t)) j ps) V _ _ :=
@@ -106,6 +150,5 @@ Section Packaging.
     {| Preproof.rpp_proof := preproof_of b;
        Preproof.rpp_root := root;
        Preproof.rpp_root_in := _ |}.
-  Next Obligation.
-  Admitted.
+  Admit Obligations.
 End Packaging.
